WfType changed to be more ideomatic

WfType.v
@@ -2,32 +2,77 @@ From mathcomp Require Import ssreflect ssrfun ssrbool ssrnat seq fintype.
 From mathcomp Require Import eqtype fingraph path order. 
 From event_struct Require Import utilities.
 
-Import Order.TTheory.
+Set Implicit Arguments.
+Unset Strict Implicit.
+Unset Printing Implicit Defensive.
+
+Import Order.LTheory.
 Open Scope order_scope.
 
 Notation ordType := (orderType tt).
 
 Section WfDef.
 
-Variable T : ordType.
+Context {T : Type} (r : rel T).
 
-Inductive acc (x : T) :=
-  acc_intro of (forall y : T, y < x -> acc y).
+Inductive acc_bool (x : T) :=
+  acc_bool_intro of (forall y : T, r y x -> acc_bool y).
 
-Definition well_founded := forall x, acc x.
+Definition well_founded_bool := forall x, acc_bool x.
 
 End WfDef.
 
-Structure wfType : Type := 
-  Well_founded {type :> ordType; #[canonical(false)] wf : well_founded type}.
+Module WellFounded.
+
+Section ClassDef.
+
+Definition mixin_of T0 (b : Order.POrder.class_of T0) (T := Order.POrder.Pack tt b) :=
+  well_founded_bool (<%O : rel T).
+
+Set Primitive Projections.
+
+Record class_of (T : Type) := Class {
+  base  : Order.POrder.class_of T;
+  mixin : mixin_of base;
+}.
+
+Unset Primitive Projections.
+
+Local Coercion base : class_of >-> Order.POrder.class_of.
+
+Structure type (disp : unit) := Pack { sort; _ : class_of sort }.
+
+Local Coercion sort : type >-> Sortclass.
+
+Variables (T : Type) (disp : unit) (cT : type disp).
+
+Definition class := let: Pack _ c as cT' := cT return class_of cT' in c.
+
+Definition porderType := @Order.POrder.Pack disp cT class.
+
+End ClassDef.
+
+Coercion base : class_of >-> Order.POrder.class_of.
+Coercion sort : type >-> Sortclass.
+Coercion porderType : type >-> Order.POrder.type.
+Canonical porderType.
+
+End WellFounded.
+
+Notation wfType := (WellFounded.type tt).
+
+Import WellFounded.
 
 Section WfInduction.
 
 Context {T : wfType}.
 
+Lemma wf : well_founded_bool (<%O : rel T).
+Proof. by case: T=> ? []. Qed.
+
 Lemma wf_ind (P : T -> Type) :
   (forall n, (forall m, m < n -> P m) -> P n) ->
   forall n, P n.
-Proof. move=> accP M. by elim: (wf _ M) => ?? /accP. Qed.
+Proof. move=> accP M. by elim: (wf M) => ?? /accP. Qed.
 
 End  WfInduction.
